```
These matrices are for primitive variables
*********************************************************************

ke = (u[0]*u[0] + u[1]*u[1] + u[2]*u[2])/2               //kinetic energy 
---------------------------------------

Ai_1[5][5] = {0}

Ai_1[0][1] = 1

Ai_1[1][0] = -u[0]*u[0] + ke*Rd/cv
Ai_1[1][1] = u[0] * (2 - Rd/cv)
Ai_1[1][2] = -Rd*u[1]/cv
Ai_1[1][3] = -Rd*u[2]/cv
Ai_1[1][4] = Rd/cv

Ai_1[2][0] = -u[0]*u[1]
Ai_1[2][1] = u[1]
Ai_1[2][2] = u[0]

Ai_1[3][0] = -u[0]*u[2]
Ai_1[3][1] = u[2]
Ai_1[3][3] = u[0]

Ai_1[4][0] = u[0] * ( 2*Rd*ke/cv - E * (Rd/cv + 1) )
Ai_1[4][1] = E * (Rd/cv + 1) - Rd * (u[0]*u[0] + ke)/cv
Ai_1[4][2] = -Rd*u[0]*u[1]/cv
Ai_1[4][3] = -Rd*u[0]*u[2]/cv
Ai_1[4][4] = u[0] * (Rd/cv + 1)

****************

Ai_2[5][5] = {0}

Ai_2[0][2] = 1


Ai_2[1][0] = -u[1]*u[0]
Ai_2[1][1] = u[1]
Ai_2[1][2] = u[0]

Ai_2[2][0] = -u[1]*u[1] + ke*Rd/cv
Ai_2[2][1] = -Rd*u[0]/cv
Ai_2[2][2] = u[1] * (2 - Rd/cv)
Ai_2[2][3] = -Rd*u[2]/cv
Ai_2[2][4] = Rd/cv

Ai_2[3][0] = -u[1]*u[2]
Ai_2[3][2] = u[2]
Ai_2[3][3] = u[1]

Ai_2[4][0] = u[1] * ( 2*Rd*ke/cv - E * (Rd/cv + 1) )
Ai_2[4][1] = -Rd*u[1]*u[0]/cv
Ai_2[4][2] = E * (Rd/cv + 1) - Rd * (u[1]*u[1] + ke)/cv
Ai_2[4][3] = -Rd*u[1]*u[2]/cv
Ai_2[4][4] = u[1] * (Rd/cv + 1)

****************

Ai_3[5][5] = {0}

Ai_3[0][3] = 1

Ai_3[1][0] = -u[2]*u[0]
Ai_3[1][1] = u[2]
Ai_3[1][3] = u[0]

Ai_3[2][0] = -u[2]*u[1]
Ai_3[2][2] = u[2]
Ai_3[2][3] = u[1]

Ai_3[3][0] = -u[2]*u[2] + ke*Rd/cv
Ai_3[3][1] = -Rd*u[0]/cv
Ai_3[3][2] = -Rd*u[1]/cv
Ai_3[3][3] = u[2] * (2 - Rd/cv)
Ai_3[3][4] = Rd/cv

Ai_3[4][0] = u[2] * ( 2*Rd*ke/cv - E * (Rd/cv + 1) )
Ai_3[4][1] = -Rd*u[2]*u[0]/cv
Ai_3[4][2] = -Rd*u[2]*u[1]/cv
Ai_3[4][3] = E * (Rd/cv + 1) - Rd * (u[2]*u[2] + ke)/cv
Ai_3[4][4] = u[2] * (Rd/cv + 1)
*********************************************************************

f1 = rho * sqrt( 2/dt + < u^T * u , BB >,F ) 
TauC = f1/( 8 * (BB[0] + BB[3] + BB[5]) ) 
TauM = 1/f1  
TauE = 1/(f1*cv)     
--------------------------------------------

Tau[5][5] = {0}

Tau[0][0] = TauC
Tau[1][1] = TauM
Tau[2][2] = TauM
Tau[3][3] = TauM
Tau[4][4] = TauE

*********************************************************************
//Body Force
F[5] = {0, 0, 0, rho*g, rho*g*u[2]}
*********************************************************************

//Aj * U,j 






```